-correctness of TM nearly complete -added more towards step-analysis of LAM

theories/LAM/TM/SizeAnalysis.v
@@ -3,27 +3,23 @@ From Undecidability.L Require Import LM_heap_def.
 
 Require Import FunInd.
 
-Fixpoint sum (A:list nat) :=
-  match A with
-    [] => 0
-  | a::A => a + sum A
-  end.
-
-Lemma sum_app A B : sum (A++B) = sum A + sum B.
-Proof.
-  induction A;cbn;omega.
-Qed.
-
-Hint Rewrite sum_app : list. 
-
 Definition sizeT t := 
     match t with
       varT n => 1 + n
     |  _ => 1
     end.  
 
-Definition sizeP (P:Pro) := 1 + sum (map sizeT P).
-Hint Unfold sizeP.   
+Definition sizeP (P:Pro) := 1 + sumn (map sizeT P).
+Hint Unfold sizeP : core.
+
+Lemma lookup_el H alpha x c: lookup H alpha x = Some c -> exists beta, Some (c,beta) el H.
+Proof.
+  induction x in alpha, c|-*.
+  all:cbn. all:destruct nth_error as [[[] | ]| ] eqn:eq.
+  all:intros [= eq'].
+  1:subst.
+  all:eauto using nth_error_In.
+Qed.
 
 Section Analysis.
 
@@ -31,7 +27,7 @@ Section Analysis.
   (*Variable s : term.*)
  (* Hypothesis cs : closed s.*)
   Variable T V : list HClos.
-  Variable H: list HEntr.
+  Variable H H__init: list HEntr.
 
   Lemma jumpTarget_eq c c0 c1 c2: jumpTarget 0 c0 c = Some (c1,c2) -> c1++[retT]++c2=c0++c.
   Proof.
@@ -44,23 +40,26 @@ Section Analysis.
     all:now cbn in *. 
   Qed.
 
-(*
-  Lemma tailRecursion_incl c alpha T': tailRecursion c alpha T' <<= c!alpha::T'.
+
+  Lemma tailRecursion_incl P alpha T': tailRecursion (alpha,P) T' <<= (alpha,P)::T'.
   Proof.
-    destruct c as [|[]];cbn. all:eauto.
+    destruct P as [ |[]];cbn. all:eauto.
   Qed.
 
-  Lemma tailRecursion_length c alpha T': | tailRecursion c alpha T'| <= 1+ length T'.
+  Lemma tailRecursion_length P alpha T': | tailRecursion (alpha,P) T' | <= 1+ length T'.
   Proof.
-    destruct c as [|[]];cbn. all:eauto.
+    destruct P as [ |[]];cbn. all:eauto.
   Qed.
-*)
+
   
   Variable i : nat.
 
   Variable P0 : Pro.
-  Hypothesis R: pow step i ([(0,P0)],[],[None]) (T,V,H).
+  Hypothesis R: pow step i ([(0,P0)],[],H__init) (T,V,H).
+  Hypothesis empty_H__init: forall c, c el H__init -> c = None.
 
+  Import Lia.
+  
   Lemma size_clos P a : ((a,P) el (T++V) -> sizeP P <= sizeP P0 /\ a <= length H)
                         /\ (forall beta, Some ((a,P),beta) el H -> sizeP P <= sizeP P0 /\ a <= length H /\ beta <= length H).
   Proof.
@@ -69,24 +68,24 @@ Section Analysis.
     -inv R. split.
      +intros [[= <- <-]|[]].
       eauto using Nat.le_0_l.
-     +intros ? [H|[]]. inv H.
-    -(*apply pow_add in R. destruct R as [[[T' V'] H'] [R1 R2]].
+     +intros ? ?%empty_H__init. easy.
+    -replace (S n) with (n + 1) in R by lia. apply pow_add in R. destruct R as [[[T' V'] H'] [R1 R2]].
      specialize (IHn _ _ _ R1).
      eapply rcomp_1 in R2.
      split.
      +intros Hel.
-      apply in_app_or in Hel.
+      apply in_app_or in Hel. 
       inv R2.
       *apply jumpTarget_eq in H2.  cbn in H2;inv H2.
        destruct Hel as [H1|[[= <- <-] | ]].
-       apply tailRecursion_incl in H1 as [[= <- <-]|].
+       apply tailRecursion_incl in H1 as [[= <- <-]| ].
        
        all:repeat (autorewrite with list in *;cbn in * ).
        1:specialize (proj1 (IHn _ a0) ltac:(eauto)).
        3:specialize (proj1 (IHn _ a0) ltac:(eauto)).
        
        1,3:repeat (autorewrite with list in *;cbn in * ).
-       1,2:omega.
+       1,2:split;try nia.
 
        1:specialize (proj1 (IHn P a) ltac:(eauto)).
        2:specialize (proj1 (IHn P a) ltac:(eauto)).
@@ -94,8 +93,8 @@ Section Analysis.
        all:omega.
 
       *inv H2.
-       destruct Hel as [[[= <- <-] | ]|].
-       2:apply tailRecursion_incl in H as [[= <- <-]|].
+       destruct Hel as [[[= <- <-] | ]| ].
+       2:apply tailRecursion_incl in H as [[= <- <-]| ].
        all:repeat ((try setoid_rewrite in_app_iff in IHn);cbn in IHn).
        1:specialize (proj1(IHn Q _) ltac:(eauto)).
        1:repeat (autorewrite with list in *;cbn in * ).
@@ -114,8 +113,8 @@ Section Analysis.
        1:autorewrite with list in IHn.
        1:repeat (autorewrite with list in *;cbn in * ).
        1:try now omega.
-      *destruct Hel as [|[-> | ]].
-       apply tailRecursion_incl in H0 as [[= <- <-]|].
+      *destruct Hel as [ |[-> | ]].
+       apply tailRecursion_incl in H0 as [[= <- <-]| ].
 
        all:repeat ((try setoid_rewrite in_app_iff in IHn);cbn in IHn).
        1:specialize (proj1(IHn _ a0) ltac:(eauto)).
@@ -138,43 +137,43 @@ Section Analysis.
       1,3:now apply IHn.
       inv H2.
       apply in_app_or in Hel.
-      edestruct Hel as [|[[= -> ->]|[]]].
+      edestruct Hel as [ |[[= -> ->]|[]]].
       1:specialize (proj2(IHn _ a) _ ltac:(eauto)).
       all:autorewrite with list;cbn.
       now omega.
       1:specialize (proj1(IHn _ a) ltac:(eauto)).
       1:specialize (proj1(IHn _ beta) ltac:(eauto)).
-      omega.*)
-  Admitted.
+      omega.
+  Qed.
 
-  Lemma length_H : length H <= 1+i.
+  Lemma length_H : length H <= length H__init+i.
   Proof.
     induction i in T,V,H,R|-*.
     -inv R. cbn;omega.
     -replace (S n) with (n + 1) in R by omega.
-     (*
      apply pow_add in R. destruct R as [[[T' V'] H'] [R1 R2]].
      specialize (IHn _ _ _ R1).
      eapply rcomp_1 in R2.
      inv R2.
      1,3:now omega.
-     inv H2. autorewrite with list. cbn. omega.*)
-  Admitted.
+     inv H2. autorewrite with list. cbn. omega.
+  Qed.
 
   Lemma length_TV : length T + length V <= 1+i.
   Proof.
     induction i in T,V,H,R|-*.
     -inv R. cbn;omega.
     -replace (S n) with (n + 1) in R by omega.
-     (*apply pow_add in R. destruct R as [[[T' V'] H'] [R1 R2]].
+     apply pow_add in R. destruct R as [[[T' V'] H'] [R1 R2]].
      specialize (IHn _ _ _ R1).
      eapply rcomp_1 in R2.
      inv R2.
      all:cbn in *.
-     specialize (tailRecursion_length P' a T0). omega.
-     1,2:specialize (tailRecursion_length P a T0).
-     1,2:omega.*)
-  Admitted.
+     specialize (tailRecursion_length P' a T0). 
+     1,2:specialize (tailRecursion_length P a T0). all:unfold tailRecursion.
+     1,2:nia.
+     destruct P. nia. cbn. nia.
+  Qed.
   
 (* Damit: länge eines zustandes beschränkt durch (i+i)*(3*(i+1)+2*|s|)*)
   
