theories/LAM/TM/LMBounds_Loop.v
@@ -1,0 +1,79 @@
+
+From Undecidability Require Import TM.PrettyBounds.PrettyBounds.
+From Undecidability Require Import TM.PrettyBounds.BaseCode.
+From Undecidability Require Import LM_heap_def TM.PrettyBounds.MaxList.
+
+From Undecidability.LAM Require Import TM.Alphabets.
+From Undecidability.LAM.TM Require Import CaseCom.
+From Undecidability.LAM.TM Require Import StepTM LMBounds HaltingProblem.
+
+From Undecidability Require Import UpToCNary.
+Print Loop_steps.
+Check LM.Step_steps_nice.
+
+
+
+Lemma sizeT_ge_1 t:
+  1 <= sizeT t.
+Proof.
+  destruct t;cbn. all:nia.
+Qed.
+
+Lemma size_sizeT_le t:
+  size t <= 2* sizeT t.
+Proof.
+  destruct t.
+  1:rewrite size_Var.
+  all:cbv - [plus mult]. all:nia.
+Qed.
+
+Lemma size_le_sizeP P:
+  size P <= 3 * sizeP P.
+Proof.
+  induction P as [ | t P].
+  {now cbv. }
+  setoid_rewrite encodeList_size_cons. rewrite IHP.
+  unfold sizeP;cbn. rewrite size_sizeT_le.
+  specialize (sizeT_ge_1 t). nia.
+Qed.
+(*
+Lemma sizeH_le H:
+  size H <= 
+Proof.
+  induction P as [ | t P].
+  {now cbv. }
+  setoid_rewrite encodeList_size_cons. rewrite IHP.
+  unfold sizeP;cbn. rewrite size_sizeT_le.
+  specialize (sizeT_ge_1 t). nia.
+Qed.
+*)  
+
+Section FixInit.
+
+  Variable T V : list HClos.
+  Variable H H__init: list HEntr.
+  Variable i : nat.
+
+  Variable P0 : Pro.
+  Hypothesis R: pow step i ([(0,P0)],[],H__init) (T,V,H).
+  Hypothesis empty_H__init: forall c, c el H__init -> c = None.
+  (*
+  Lemma Step_steps_nice :
+    {c : nat |
+      forall (T V : list HClos) (H : Heap),
+        pow step i ([(0,P0)],[],H__init) (T,V,H)
+        -> Step_steps T V H <=(c) (let a := length H__init + i in
+                                 1 + a + 
+                                size a + size H + size V +
+                                size P * (1 + size H + Init.Nat.max a (LM_Lookup_nice.heap_greatest_address2 H) + size P)
+                              end}.
+
+Lemma Loop_steps_nice' :
+  (fun '(T,V,H,k) => Loop_steps [c] [] [] k) <=c (fun '(T,V,H,k) => 1).
+Proof.
+
+Lemma Loop_steps_nice :
+  (fun '(T,V,H,k) => Loop_steps [c] [] [] k) <=c (fun '(T,V,H,k) => 1).
+Proof.
+   *)
+End FixInit.
